symbolic/fault_handler.v
@@ -190,7 +190,7 @@ Definition handler : code :=
 Section invariant.
 
 Context {s : machine_ops_spec ops}
-        {ap : Symbolic.symbolic_params}
+        {ap : Symbolic.params}
         {e : encodable Symbolic.tag}.
 
 Record policy_invariant : Type := {
